lib/Lib.ByteVector.fsti
@@ -1,0 +1,107 @@
+module Lib.ByteVector
+
+open FStar.Mul
+open Lib.Sequence
+open Lib.IntTypes
+open Lib.IntVector
+
+module BSeq = Lib.ByteSequence
+module LSeq = Lib.Sequence
+
+#set-options "--z3rlimit 20 --max_fuel 0 --max_ifuel 0"
+
+inline_for_extraction noextract
+val vecs_from_bytes_le: vt:v_inttype -> w:width -> len:nat{len * (numbytes vt * w) <= max_size_t}
+  -> b:lseq uint8 (len * (numbytes vt * w)) -> lseq (vec_t vt w) len
+
+val index_vecs_from_bytes_le: vt:v_inttype -> w:width -> len:nat{len * (numbytes vt * w) <= max_size_t}
+  -> b:lseq uint8 (len * (numbytes vt * w)) -> i:nat{i < len} ->
+  Lemma ((vecs_from_bytes_le vt w len b).[i] == vec_from_bytes_le vt w (LSeq.sub b (i * (numbytes vt * w)) (numbytes vt * w)))
+
+
+inline_for_extraction noextract
+val vecs_from_bytes_be: vt:v_inttype -> w:width -> len:nat{len * (numbytes vt * w) <= max_size_t}
+  -> b:lseq uint8 (len * (numbytes vt * w)) -> lseq (vec_t vt w) len
+
+val index_vecs_from_bytes_be: vt:v_inttype -> w:width -> len:nat{len * (numbytes vt * w) <= max_size_t}
+  -> b:lseq uint8 (len * (numbytes vt * w)) -> i:nat{i < len} ->
+  Lemma ((vecs_from_bytes_be vt w len b).[i] == vec_from_bytes_be vt w (LSeq.sub b (i * (numbytes vt * w)) (numbytes vt * w)))
+
+inline_for_extraction noextract
+val vecs_to_bytes_le: #vt:v_inttype -> #w:width -> #len:nat{len * (numbytes vt * w) <= max_size_t}
+  -> vl:lseq (vec_t vt w) len -> lseq uint8 (len * (numbytes vt * w))
+
+val index_vecs_to_bytes_le: #vt:v_inttype -> #w:width -> #len:nat{len * (numbytes vt * w) <= max_size_t}
+  -> vl:lseq (vec_t vt w) len -> i:nat{i < len * (numbytes vt * w)} ->
+  Lemma ((vecs_to_bytes_le #vt #w #len vl).[i] == (vec_to_bytes_le vl.[i / (numbytes vt * w)]).[i % (numbytes vt * w)])
+
+inline_for_extraction noextract
+val vecs_to_bytes_be: #vt:v_inttype -> #w:width -> #len:nat{len * (numbytes vt * w) <= max_size_t}
+  -> vl:lseq (vec_t vt w) len -> lseq uint8 (len * (numbytes vt * w))
+
+val index_vecs_to_bytes_be: #vt:v_inttype -> #w:width -> #len:nat{len * (numbytes vt * w) <= max_size_t}
+  -> vl:lseq (vec_t vt w) len -> i:nat{i < len * (numbytes vt * w)} ->
+  Lemma ((vecs_to_bytes_be #vt #w #len vl).[i] == (vec_to_bytes_be vl.[i / (numbytes vt * w)]).[i % (numbytes vt * w)])
+
+
+open Lib.Buffer
+open FStar.HyperStack
+open FStar.HyperStack.ST
+module B = Lib.Buffer
+module ST = FStar.HyperStack.ST
+
+
+inline_for_extraction noextract
+val vecs_load_le:
+    #vt:v_inttype
+  -> #w:width
+  -> #len:size_t{v len * (numbytes vt * w) <= max_size_t}
+  -> o:lbuffer (vec_t vt w) len
+  -> i:lbuffer uint8 (len *! (size (numbytes vt) *! size w)) ->
+  Stack unit
+    (requires fun h -> live h i /\ live h o /\ B.disjoint i o)
+    (ensures  fun h0 _ h1 ->
+      modifies1 o h0 h1 /\
+      as_seq h1 o == vecs_from_bytes_le vt w (v len) (as_seq h0 i))
+
+
+inline_for_extraction noextract
+val vecs_load_be:
+    #vt:v_inttype
+  -> #w:width
+  -> #len:size_t{v len * (numbytes vt * w) <= max_size_t}
+  -> o:lbuffer (vec_t vt w) len
+  -> i:lbuffer uint8 (len *! (size (numbytes vt) *! size w)) ->
+  Stack unit
+    (requires fun h -> live h i /\ live h o /\ B.disjoint i o)
+    (ensures  fun h0 _ h1 ->
+      modifies1 o h0 h1 /\
+      as_seq h1 o == vecs_from_bytes_be vt w (v len) (as_seq h0 i))
+
+
+inline_for_extraction noextract
+val vecs_store_le:
+    #vt:v_inttype
+  -> #w:width
+  -> #len:size_t{v len * (numbytes vt * w) <= max_size_t}
+  -> o:lbuffer uint8 (len *! (size (numbytes vt) *! size w))
+  -> i:lbuffer (vec_t vt w) len ->
+  Stack unit
+    (requires fun h -> live h i /\ live h o /\ B.disjoint i o)
+    (ensures  fun h0 _ h1 ->
+      modifies1 o h0 h1 /\
+      as_seq h1 o == vecs_to_bytes_le #vt #w #(v len) (as_seq h0 i))
+
+
+inline_for_extraction noextract
+val vecs_store_be:
+    #vt:v_inttype
+  -> #w:width
+  -> #len:size_t{v len * (numbytes vt * w) <= max_size_t}
+  -> o:lbuffer uint8 (len *! (size (numbytes vt) *! size w))
+  -> i:lbuffer (vec_t vt w) len ->
+  Stack unit
+    (requires fun h -> live h i /\ live h o /\ B.disjoint i o)
+    (ensures  fun h0 _ h1 ->
+      modifies1 o h0 h1 /\
+      as_seq h1 o == vecs_to_bytes_be #vt #w #(v len) (as_seq h0 i))
